Prove the correctness of Captures

correctness/RegexCorrectness/Regex/Iterators/Captures.lean
@@ -2,21 +2,20 @@ import Regex.Regex.Iterators.Captures
 import RegexCorrectness.Regex.Iterators.CapturedGroups
 
 open String (Pos)
+open Std.Iterators
 
 namespace Regex.Captures
 
 def Valid (self : Captures) : Prop :=
-  self.regex.IsSearchRegex ∧ self.bufferSize = self.regex.maxTag + 1 ∧ self.currentPos.ValidPlus self.haystack
+  self.regex.IsSearchRegex ∧ self.currentPos.ValidPlus self.haystack
 
-theorem valid_of_yield_valid {self self' : Captures} {groups : CapturedGroups} (h : self.step = .yield self' groups)
+theorem valid_yield_of_valid {self self' : Captures} {groups : CapturedGroups} (h : self.step = .yield self' groups)
   (v : self.Valid) :
-  self'.Valid ∧ groups.Spec v.1 self.haystack self.currentPos := by
+  self'.Valid := by
   have ⟨hle, buffer, eq₁, eq₂, matched, eq₃, eq₄⟩ := step_yield self self' groups h
-  have v' := v.2.2.valid_of_le hle
+  have v' := v.2.valid_of_le hle
   have ⟨it, it', groups', eqs, le, c, eqv, eq₅, eq₆⟩ := v.1.captureNextBuf_soundness eq₁ v' (by simp)
-  refine ⟨⟨?_, ?_, ?_⟩, ?_⟩
-  . simpa [eq₄] using v.1
-  . simpa [eq₄] using v.2.1
+  refine ⟨by simpa [eq₄] using v.1, ?_⟩
   . simp [eq₄]
     split
     next =>
@@ -26,31 +25,122 @@ theorem valid_of_yield_valid {self self' : Captures} {groups : CapturedGroups} (
       simp [↓eqs] at vp
       exact vp
     next => exact String.Pos.validPlus_of_next_valid v'
-  . refine ⟨it, it', groups', by simp [↓eqs], le, c, ?_, ?_⟩
-    . simp [eq₂, CapturedGroups.get, eq₅, eq₆]
-    . intro i p₁ p₂
-      if lt : 2 * i + 1 < max self.bufferSize 2 then
-        have h := eqv.eq i lt p₁ p₂
-        simp [h, eq₂, CapturedGroups.get, Option.bind_eq_some_iff, Vector.getElem_eq_iff]
-      else
-        have eqsize : groups.buffer.size = max self.bufferSize 2 := by
-          simp [eq₂]
-        have eq : groups.get i = .none := groups.get_eq_none_of_ge (Nat.ge_of_not_lt (eqsize ▸ lt))
-        simp [eq]
-        intro eq'
-        have mem : i ∈ v.1.expr.tags := Strategy.mem_tags_of_materializeRegexGroups_some (tag := i) c (by simp [eq'])
-        have lt' : 2 * i < self.regex.maxTag := v.1.maxTag_eq ▸ NFA.lt_of_mem_tags_compile v.1.nfa_eq.symm mem
-        have eqBufSize : self.bufferSize = self.regex.maxTag + 1 := v.2.1
-        omega
 
-theorem valid_of_skip_valid {self self' : Captures} (h : self.step = .skip self') (v : self.Valid) :
+theorem spec_yield_of_valid_of_bufferSize_eq {self self' : Captures} {groups : CapturedGroups} (h : self.step = .yield self' groups)
+  (v : self.Valid) (eqBufSize : self.bufferSize = self.regex.maxTag + 1) :
+  groups.Spec v.1 self.haystack self.currentPos := by
+  have ⟨hle, buffer, eq₁, eq₂, matched, eq₃, eq₄⟩ := step_yield self self' groups h
+  have v' := v.2.valid_of_le hle
+  have ⟨it, it', groups', eqs, le, c, eqv, eq₅, eq₆⟩ := v.1.captureNextBuf_soundness eq₁ v' (by simp)
+  refine ⟨it, it', groups', by simp [↓eqs], le, c, ?_, ?_⟩
+  . simp [eq₂, CapturedGroups.get, eq₅, eq₆]
+  . intro i p₁ p₂
+    if lt : 2 * i + 1 < max self.bufferSize 2 then
+      have h := eqv.eq i lt p₁ p₂
+      simp [h, eq₂, CapturedGroups.get, Option.bind_eq_some_iff, Vector.getElem_eq_iff]
+    else
+      have eqsize : groups.buffer.size = max self.bufferSize 2 := by
+        simp [eq₂]
+      have eq : groups.get i = .none := groups.get_eq_none_of_ge (Nat.ge_of_not_lt (eqsize ▸ lt))
+      simp [eq]
+      intro eq'
+      have mem : i ∈ v.1.expr.tags := Strategy.mem_tags_of_materializeRegexGroups_some (tag := i) c (by simp [eq'])
+      have lt' : 2 * i < self.regex.maxTag := v.1.maxTag_eq ▸ NFA.lt_of_mem_tags_compile v.1.nfa_eq.symm mem
+      omega
+
+theorem valid_skip_of_valid {self self' : Captures} (h : self.step = .skip self') (v : self.Valid) :
   self'.Valid := by
   have ⟨hle, h⟩ := step_skip self self' h
-  have v' := v.2.2.valid_of_le hle
-  exact ⟨by simpa [h] using v.1, by simpa [h] using v.2.1, by simp [h, String.Pos.ValidPlus]⟩
+  have v' := v.2.valid_of_le hle
+  exact ⟨by simpa [h] using v.1, by simp [h, String.Pos.ValidPlus]⟩
 
-theorem valid_captures {re : Regex} (haystack : String) (s : re.IsSearchRegex) :
-  (re.captures haystack).internalState.Valid :=
-  ⟨s, rfl, haystack.valid_mkIterator.validPlus⟩
+namespace IterM
+
+variable {m : Type → Type w} [Pure m] {it' it : IterM (α := Captures) m CapturedGroups} {out : CapturedGroups}
+
+theorem valid_capturesM {re : Regex} (haystack : String) (m : Type → Type w) (bufferSize : Nat) (s : re.IsSearchRegex) :
+  (re.capturesM haystack m bufferSize).internalState.Valid :=
+  ⟨s, haystack.valid_mkIterator.validPlus⟩
+
+theorem valid_of_isPlausibleSuccessorOf_of_valid (so : it'.IsPlausibleSuccessorOf it) (v : it.internalState.Valid) :
+  it'.internalState.Valid := by
+  obtain ⟨step, h, h'⟩ := so
+  simp [IterM.IsPlausibleStep, Iterator.IsPlausibleStep, IsPlausibleStep] at h'
+  cases eq : it.internalState.step with
+  | yield it' out =>
+    simp [eq] at h'
+    simp [h', IterStep.successor] at h
+    simp [←h]
+    exact valid_yield_of_valid eq v
+  | skip it' =>
+    simp [eq] at h'
+    simp [h', IterStep.successor] at h
+    simp [←h]
+    exact valid_skip_of_valid eq v
+  | done =>
+    simp [eq] at h'
+    simp [h', IterStep.successor] at h
+
+theorem eq_withPos_of_isPlausibleSuccessorOf (so : it'.IsPlausibleSuccessorOf it) :
+  ∃ pos, it'.internalState = it.internalState.withPos pos := by
+  obtain ⟨step, h, h'⟩ := so
+  simp [IterM.IsPlausibleStep, Iterator.IsPlausibleStep, IsPlausibleStep] at h'
+  cases eq : it.internalState.step with
+  | yield it' out =>
+    simp [eq] at h'
+    simp [h', IterStep.successor] at h
+    have ⟨_, _, _, _, _, _, eq₄⟩ := step_yield it.internalState it' out eq
+    simp [←h, eq₄]
+  | skip it' =>
+    simp [eq] at h'
+    simp [h', IterStep.successor] at h
+    have ⟨_, h''⟩ := step_skip it.internalState it' eq
+    simp [←h, h'']
+  | done =>
+    simp [eq] at h'
+    simp [h', IterStep.successor] at h
+
+theorem spec_of_isPlausibleOutput_of_valid_of_bufferSize_eq (o : it.IsPlausibleOutput out) (v : it.internalState.Valid)
+  (eqBufSize : it.internalState.bufferSize = it.internalState.regex.maxTag + 1) :
+  out.Spec v.1 it.internalState.haystack it.internalState.currentPos := by
+  obtain ⟨it', h⟩ := o
+  simp [IterM.IsPlausibleStep, Iterator.IsPlausibleStep, IsPlausibleStep] at h
+  cases eq : it.internalState.step with
+  | yield _ groups =>
+    simp [eq] at h
+    simp [h]
+    exact spec_yield_of_valid_of_bufferSize_eq eq v eqBufSize
+  | skip _ | done => simp [eq] at h
+
+theorem spec_of_isPlausibleIndirectOutput_of_valid_of_bufferSize_eq (io : it.IsPlausibleIndirectOutput out) (v : it.internalState.Valid)
+  (eqBufSize : it.internalState.bufferSize = it.internalState.regex.maxTag + 1) :
+  ∃ startPos, out.Spec v.1 it.internalState.haystack startPos := by
+  induction io with
+  | @direct it out h => exact ⟨it.internalState.currentPos, spec_of_isPlausibleOutput_of_valid_of_bufferSize_eq h v eqBufSize⟩
+  | @indirect it it' out so io ih =>
+    have ih := ih (valid_of_isPlausibleSuccessorOf_of_valid so v)
+    have ⟨pos, eq⟩ := eq_withPos_of_isPlausibleSuccessorOf so
+    simp [eq] at ih
+    exact ih eqBufSize
+
+end IterM
+
+namespace Iter
+
+theorem valid_captures {re : Regex} (haystack : String) (bufferSize : Nat) (s : re.IsSearchRegex) :
+  (re.captures haystack bufferSize).internalState.Valid :=
+  IterM.valid_capturesM haystack Id bufferSize s
+
+theorem spec_of_isPlausibleIndirectOutput_of_captures {re : Regex} (haystack : String) (s : re.IsSearchRegex)
+  (io : (re.captures haystack).IsPlausibleIndirectOutput out) :
+  ∃ startPos, out.Spec s haystack startPos := by
+  have v : (re.captures haystack).internalState.Valid := valid_captures haystack (re.maxTag + 1) s
+  have eqBufSize : (re.captures haystack).internalState.bufferSize = re.maxTag + 1 := rfl
+  rw [Iter.isPlausibleIndirectOutput_iff_isPlausibleIndirectOutput_toIterM] at io
+  exact IterM.spec_of_isPlausibleIndirectOutput_of_valid_of_bufferSize_eq io v eqBufSize
+
+-- TODO: Iter.isPlausibleIndirectOutput_of_mem_toArray
+
+end Iter
 
 end Regex.Captures
