correctness/RegexCorrectness/Regex/Iterators/Matches.lean
@@ -1,4 +1,4 @@
-import Regex.Regex.Matches
+import Regex.Regex.Iterators.Matches
 import RegexCorrectness.Regex.Basic
 
 set_option autoImplicit false
@@ -22,65 +22,10 @@ def Spec {re : Regex} (s : re.IsSearchRegex) (haystack : String) (startPos : Pos
     s.expr.Captures it it' groups ∧
     str = ⟨haystack, it.pos, it'.pos⟩
 
-def Valid (self : Matches) : Prop :=
-  self.regex.IsSearchRegex ∧ self.currentPos.ValidPlus self.haystack
-
-theorem captures_of_next?_some {self self' : Matches} {s} (h : self.next? = .some (s, self'))
-  (v : self.Valid) :
-  self'.Valid ∧ Spec v.1 self.haystack self.currentPos s := by
-  unfold next? at h
-  split at h
-  next le =>
-    have pos_valid := v.2.valid_of_le le
-    match h' : self.regex.searchNext ⟨self.haystack, self.currentPos⟩ with
-    | none => simp [h'] at h
-    | some matched =>
-      simp [h'] at h
-      have ⟨it, it', groups, eqs, le, c, eq₁, eq₂⟩ := v.1.searchNext_some h' pos_valid
-      simp at eqs
-      refine ⟨?v', it, it', groups, eqs, le, c, ?eq⟩
-      case eq =>
-        simp [Regex.searchNext, Option.bind_eq_some_iff] at h'
-        have ⟨_, _, p₁, _, p₂, _, h'⟩ := h'
-        simp [←h'] at eq₁ eq₂
-        simp [←h.1, ←h', eq₁, eq₂]
-      case v' =>
-        split at h
-        next =>
-          simp [←h.2]
-          have vp : Pos.ValidPlus it.toString matched.stopPos := c.toString_eq ▸ eq₂ ▸ c.validR.validPlus
-          exact ⟨v.1, eqs ▸ vp⟩
-        next =>
-          simp [←h.2]
-          exact ⟨v.1, String.Pos.validPlus_of_next_valid pos_valid⟩
-  next => simp at h
-
-theorem regex_eq_of_next?_some {self self' : Matches} {positions : Substring} (h : self.next? = .some (positions, self')) :
-  self'.regex = self.regex := by
-  unfold next? at h
-  split at h
-  next =>
-    match h' : self.regex.searchNext ⟨self.haystack, self.currentPos⟩ with
-    | none => simp [h'] at h
-    | some matched =>
-      simp [h'] at h
-      split at h <;> simp [←h]
-  next => simp at h
-
-theorem haystack_eq_of_next?_some {self self' : Matches} {positions} (h : self.next? = .some (positions, self')) :
-  self'.haystack = self.haystack := by
-  unfold next? at h
-  split at h
-  next =>
-    match h' : self.regex.searchNext ⟨self.haystack, self.currentPos⟩ with
-    | none => simp [h'] at h
-    | some matched =>
-      simp [h'] at h
-      split at h <;> simp [←h]
-  next => simp at h
-
-theorem vaild_matches {re : Regex} (haystack : String) (s : re.IsSearchRegex) :
-  (re.matches haystack).Valid :=
-  ⟨s, haystack.valid_mkIterator.validPlus⟩
+-- TODO: IsPlausibleIndirectOutput for filterMap
+-- theorem spec_of_isPlausibleIndirectOutput_of_matches {re : Regex} (haystack : String) (str : Substring) (s : re.IsSearchRegex)
+--   (io : (re.matches haystack).IsPlausibleIndirectOutput str) :
+--   ∃ startPos, Spec s haystack startPos str := by
+--   sorry
 
 end Regex.Matches
